Finalize everything except the proofs

eta-expansion/theories/PCUICEtaExpansion_Defs.v
@@ -4,11 +4,11 @@
  *
  * This file contains the definitions for eta-expansion of constructors.
  * The basic idea is quite simple:
- *    Iterate over the PCUIC AST until you find an constructor,
- *    then call the actual eta-expansion on that constructor.
+ * > Iterate over the PCUIC AST until you find an constructor,
+ * > then call the actual eta-expansion on that constructor.
  *
  * The eta-expansion itself works by recursively adding lambda abstractions
- * for each of the arguments. For example:
+ * for each of the argument types. For example:
  *
  *   current term                 | remaining type
  *  ------------------------------+--------------------------------------------
@@ -27,15 +27,12 @@ From MetaCoq.SafeChecker Require Import PCUICSafeRetyping.
 
 From Coq Require Import Program ssreflect.
 
-(** Haskell's $ notation can come in handy *)
-Notation "f $ a" := (f a) (at level 50).
-
 (** ** The actual η-expansion *)
 Section EtaExpansion.
 
   Fixpoint eta_expand (t T : term) : term :=
     match T with
-    | tProd na A B => tLambda na A $ eta_expand (tApp (lift0 1 t) (tRel 0)) B
+    | tProd na A B => tLambda na A (eta_expand (tApp (lift0 1 t) (tRel 0)) B)
     | _            => t
     end.
 
@@ -46,45 +43,46 @@ Section Transformation.
 
   Local Existing Instance extraction_checker_flags.
 
-  Section TransBrs.
-    Context (trans : forall (Σ : global_env_ext) (Γ : context) (HΣ : ∥ wf_ext Σ ∥) (t : term) (Ht : welltyped Σ Γ t), term).
+  Context (Σ : global_env_ext) (HΣ : ∥ wf_ext Σ ∥).
 
-    Definition trans_brs Σ Γ HΣ (brs : list (nat * term))
+  Section TransBrs.
+    Context (trans : forall (Γ : context)(t : term) (Ht : welltyped Σ Γ t), term).
+
+    Definition trans_brs Γ (brs : list (nat * term))
                (H : forall d, In d brs -> welltyped Σ Γ d.2) : list (nat * term) :=
-      map_InP (fun br wt => let br' := trans Σ Γ HΣ br.2 wt in (br.1, br')) brs H.
+      map_InP (fun br wt => let br' := trans Γ br.2 wt in (br.1, br')) brs H.
   End TransBrs.
 
   Section TransMfix.
-    Context (trans : forall (Σ : global_env_ext) (Γ : context) (HΣ : ∥ wf_ext Σ ∥) (t : term) (Ht : welltyped Σ Γ t), term).
+    Context (trans : forall (Γ : context) (t : term) (Ht : welltyped Σ Γ t), term).
 
-
-    Definition trans_mfix Σ Γ HΣ (defs : mfixpoint term)
+    Definition trans_mfix Γ (defs : mfixpoint term)
                (H : forall d, In d defs -> welltyped Σ (Γ ,,, PCUICLiftSubst.fix_context defs) d.(dbody)) : mfixpoint term :=
       let Γ' := (PCUICLiftSubst.fix_context defs ++ Γ)%list in
       map_InP (fun d wt =>
-                 let dbody' := trans Σ Γ' HΣ d.(dbody) wt in
+                 let dbody' := trans Γ' d.(dbody) wt in
                  ({| dname := d.(dname); rarg := d.(rarg); dbody := dbody'; dtype := d.(dtype) |})) defs H.
   End TransMfix.
 
-  Equations? trans Σ Γ (HΣ : ∥ wf_ext Σ ∥) (tm : term) (Ht : welltyped Σ Γ tm) : term :=
+  Equations? trans Γ (tm : term) (Ht : welltyped Σ Γ tm) : term :=
     {
-      trans Σ Γ HΣ (tRel n)              Ht => tRel n ;
-      trans Σ Γ HΣ (tVar i)              Ht => tVar i ;
-      trans Σ Γ HΣ (tEvar n l)           Ht => tEvar n $ map_InP (trans Σ Γ HΣ) l _ ;
-      trans Σ Γ HΣ (tSort u)             Ht => tSort u ;
-      trans Σ Γ HΣ (tProd na A B)        Ht => tProd na $ trans Σ Γ HΣ A _ $ trans Σ (vass na A :: Γ) HΣ B _ ;
-      trans Σ Γ HΣ (tLambda na A t)      Ht => tLambda na $ trans Σ Γ HΣ A _ $ trans Σ (vass na A :: Γ) HΣ t _ ;
-      trans Σ Γ HΣ (tLetIn na b B t)     Ht => tLetIn na $ trans Σ Γ HΣ b _ $ trans Σ Γ HΣ B _ $ trans Σ (vdef na b B :: Γ) HΣ t _ ;
-      trans Σ Γ HΣ (tApp u v)            Ht => tApp $ trans Σ Γ HΣ u _ $ trans Σ Γ HΣ v _ ;
-      trans Σ Γ HΣ (tConst k ui)         Ht => tConst k ui ;
-      trans Σ Γ HΣ (tInd ind ui)         Ht => tInd ind ui ;
-      trans Σ Γ HΣ (tConstruct ind n ui) Ht => let tm := tConstruct ind n ui in
+      trans Γ (tRel n)              Ht => tRel n ;
+      trans Γ (tVar i)              Ht => tVar i ;
+      trans Γ (tEvar n l)           Ht => tEvar n (map_InP (trans Γ) l _) ;
+      trans Γ (tSort u)             Ht => tSort u ;
+      trans Γ (tProd na A B)        Ht => tProd na (trans Γ A _) (trans (vass na A :: Γ) B _) ;
+      trans Γ (tLambda na A t)      Ht => tLambda na (trans Γ A _) (trans (vass na A :: Γ) t _) ;
+      trans Γ (tLetIn na b B t)     Ht => tLetIn na (trans Γ b _) (trans Γ B _) (trans (vdef na b B :: Γ) t _) ;
+      trans Γ (tApp u v)            Ht => tApp (trans Γ u _) (trans Γ v _) ;
+      trans Γ (tConst k ui)         Ht => tConst k ui ;
+      trans Γ (tInd ind ui)         Ht => tInd ind ui ;
+      trans Γ (tConstruct ind n ui) Ht => let tm := tConstruct ind n ui in
                                               let ty := type_of Σ _ _ Γ tm Ht in
                                               eta_expand tm ty ;
-      trans Σ Γ HΣ (tCase indn p c brs)  Ht => tCase indn $ trans Σ Γ HΣ p _ $ trans Σ Γ HΣ c _ $ trans_brs trans Σ Γ HΣ brs _ ;
-      trans Σ Γ HΣ (tProj p c)           Ht => tProj p $ trans Σ Γ HΣ c _ ;
-      trans Σ Γ HΣ (tFix mfix idx)       Ht => tFix $ trans_mfix trans Σ Γ HΣ mfix _ $ idx ;
-      trans Σ Γ HΣ (tCoFix mfix idx)     Ht => tCoFix $ trans_mfix trans Σ Γ HΣ mfix _ $ idx
+      trans Γ (tCase indn p c brs)  Ht => tCase indn (trans Γ p _) (trans Γ c _) (trans_brs trans Γ brs _) ;
+      trans Γ (tProj p c)           Ht => tProj p (trans Γ c _) ;
+      trans Γ (tFix mfix idx)       Ht => tFix (trans_mfix trans Γ mfix _) idx ;
+      trans Γ (tCoFix mfix idx)     Ht => tCoFix (trans_mfix trans Γ mfix _) idx
     }.
   Proof.
     all: case: HΣ => -[]* ; case: Ht => ?.
@@ -102,45 +100,55 @@ Section Transformation.
     - move=> /inversion_Case   [] //= ?. do 13 case => ?. by eexists ; eauto.
     - move=> /inversion_Case   [] //= ?. do 15 case => ?. by eexists ; eauto.
     - move=> /inversion_Case   [] //= ?. do 14 case => ?. move=> [H__brs ?].
-      eapply All2_In in H__brs as [(x' & (? & ?) & ?)]; eauto.
-      cbn in *. eexists; eauto.
+      eapply All2_In in H__brs as [(? & (? & ?) & ?)]; eauto.
+      eexists; eauto.
     - move=> /inversion_Proj   [] //= ?. do  6 case => ?. by eexists ; eauto.
     - move=> /inversion_Fix    [] //= ?. do  3 case => ?. move=> [H__fix ?].
-      eapply All_In in H__fix as [[? _]] ; eauto.
+      eapply All_In in H__fix as [[]] ; eauto.
       eexists; eauto.
-    - move=> /inversion_CoFix    [] //= ?. do  3 case => ?. move=> [H__cofix ?].
-      eapply All_In in H__cofix as [?] ; eauto.
+    - move=> /inversion_CoFix  [] //= ?. do  3 case => ?. move=> [H__cofix ?].
+      eapply All_In in H__cofix as [] ; eauto.
       eexists; eauto.
   Qed.
 
-  Program Definition trans_constant_body Σ Γ HΣ (Hwf : ∥ wf_local Σ Γ ∥) body : constant_body :=
+End Transformation.
+
+(** ** Transformation of contexts and environments *)
+Section EnvTrans.
+
+  Local Existing Instance extraction_checker_flags.
+
+  Context (Σ : global_env_ext) (HΣ : ∥ wf_ext Σ ∥).
+  Context (Γ : context) (Hwf : ∥ wf_local Σ Γ ∥).
+
+  Program Definition trans_constant_body body : constant_body :=
     if body.(cst_body) is Some tm
     then
       {|
         cst_type := body.(cst_type) ;
-        cst_body := Some $ trans Σ Γ HΣ tm _ ;
+        cst_body := Some (trans Σ HΣ Γ tm _) ;
         cst_universes := body.(cst_universes) ;
       |}
     else body.
-  Admit Obligations. (* TODO: How to use wf_local here? *)
+  Admit Obligations. (* TODO: Use wf_local to show `body.(cst_body)` is welltyped *)
 
-  Program Definition trans_context_decl Σ Γ HΣ (Hwf : ∥ wf_local Σ Γ∥) decl : context_decl :=
+  Program Definition trans_context_decl decl : context_decl :=
     if decl.(decl_body) is Some tm
     then
       {|
         decl_name := decl.(decl_name) ;
-        decl_body := Some $ trans Σ Γ HΣ tm _ ;
+        decl_body := Some (trans Σ HΣ Γ tm _) ;
         decl_type := decl.(decl_type) ;
       |}
     else decl.
-  Admit Obligations. (* TODO: How to use wf_local here? *)
+  Admit Obligations. (* TODO: Use wf_local to show `decl.(decl_body)` is welltyped *)
 
-  Definition trans_env Σ Γ HΣ Hwf :=
+  Definition trans_env :=
     let go decl := if decl is ConstantDecl b
-                   then ConstantDecl $ trans_constant_body Σ Γ HΣ Hwf b
+                   then ConstantDecl (trans_constant_body b)
                    else decl in
     (map (on_snd go) Σ.1, Σ.2).
 
-  Definition trans_ctx Σ Γ HΣ Hwf := map (trans_context_decl Σ Γ HΣ Hwf) Γ.
+  Definition trans_ctx := map trans_context_decl Γ.
 
-End Transformation.
+End EnvTrans.
